theories/lang/cpp/logic/heap_pred.v
@@ -353,11 +353,11 @@ Section with_cpp.
   (** [blockR sz q] represents [q] ownership of a contiguous chunk of
       [sz] bytes without any C++ structure on top of it. *)
   Definition blockR_def {σ} sz (q : Qp) : Rep :=
-    _offsetR (o_sub σ T_uint8 (Z.of_N sz)) validR **
-    (* ^ Encodes valid_ptr (this .[ T_uint8 ! sz]). This is
-    necessary to get [l |-> blockR n -|- l |-> blockR n ** l .[ T_uint8 ! m] |-> blockR 0]. *)
+    _offsetR (o_sub σ Tu8 (Z.of_N sz)) validR **
+    (* ^ Encodes valid_ptr (this .[ Tu8 ! sz]). This is
+    necessary to get [l |-> blockR n -|- l |-> blockR n ** l .[ Tu8 ! m] |-> blockR 0]. *)
     [∗list] i ∈ seq 0 (N.to_nat sz),
-      _offsetR (o_sub σ T_uint8 (Z.of_nat i)) (anyR (resolve:=σ) T_uint8 q).
+      _offsetR (o_sub σ Tu8 (Z.of_nat i)) (anyR (resolve:=σ) Tu8 q).
   Definition blockR_aux : seal (@blockR_def). Proof. by eexists. Qed.
   Definition blockR := blockR_aux.(unseal).
   Definition blockR_eq : @blockR = _ := blockR_aux.(seal_eq).
